hashH -> hashP

ocaml/ImpHConsOracles.ml
@@ -17,13 +17,13 @@ let make_dict (type key) (p: key Dict.hash_params) =
 
 exception Stop;;
 
-let xhCons (type a) (hh:a hashH) =
+let xhCons (type a) (hp:a hashP) =
   (* We use a hash-table, but a hash-set would be sufficient !                    *)
   (* Thus, we could use a weak hash-set, but prefer avoid it for easier debugging *)
   (* Ideally, a parameter would allow to select between the weak or full version  *)
   let module MyHashedType = struct
     type t = a hashinfo
-    let equal x y = hh.hash_eq x.hdata y.hdata
+    let equal x y = hp.hash_eq x.hdata y.hdata
     let hash x = Hashtbl.hash x.hcodes 
   end in
   let module MyHashtbl = Hashtbl.Make(MyHashedType) in
@@ -42,7 +42,7 @@ let xhCons (type a) (hh:a hashH) =
      match MyHashtbl.find_opt t k with
      | Some d -> d
      | None -> (*print_string "+";*)
-        let d = hh.set_hid k.hdata (MyHashtbl.length t) in
+        let d = hp.set_hid k.hdata (MyHashtbl.length t) in
         MyHashtbl.add t {k with hdata = d } d; d);
    next_log = (fun info -> logs := (MyHashtbl.length t, info)::(!logs));
    next_hid = (fun () -> MyHashtbl.length t);
@@ -58,7 +58,7 @@ let xhCons (type a) (hh:a hashH) =
           | (j, info)::l' when i>=j -> logs:=l'; info::(step_log i)
           | _ -> []
         in let a = Array.make (MyHashtbl.length t) k in
-           MyHashtbl.iter (fun k d -> a.(hh.get_hid d) <- k) t;
+           MyHashtbl.iter (fun k d -> a.(hp.get_hid d) <- k) t;
            {
              get_info = (fun i -> a.(i));
              iterall = (fun iter_node -> Array.iteri (fun i k -> iter_node (step_log i) i k) a)
